Complete most of the strong normalization proof

src/Norm.v
@@ -155,19 +155,43 @@ Qed.
 (** [SN] is a logical predicate that establishes the evidence needing to show
     halting. *)
 
-Equations SN {Γ τ} (e : Γ ⊢ τ) : Prop :=
-  SN (τ:=_ ⟶ _) f := f ⇓ ∧ (∀ x, SN x → SN (APP f x));
-  SN (τ:=_ × _) p := p ⇓ ∧ SN (Fst p) ∧ SN (Snd p);
-  SN e := e ⇓.
+Section Log.
 
-Lemma SN_halts {Γ τ} {e : Γ ⊢ τ} : SN e → halts e.
-Proof. intros; induction τ; simp SN in H; now reduce. Qed.
+Context {Γ : Env}.
+
+Variable P : ∀ {τ}, Exp Γ τ → Prop.
+
+Equations ExpP `(e : Exp Γ τ) : Prop :=
+  ExpP (τ:=_ ⟶ _)   f := P f ∧ (∀ x, ExpP x → ExpP (APP f x));
+  ExpP (τ:=_ × _)    p := P p ∧ ExpP (Fst p) ∧ ExpP (Snd p);
+  (* ExpP (τ:=TyList _) l := P l ∧ (∀ d, ExpP d → ExpP (Car d l)); *)
+  ExpP e := P e.
+
+Inductive SubP : ∀ {Γ'}, Sub Γ Γ' → Prop :=
+  | NoSubP : SubP (NoSub (Γ:=Γ))
+  | PushP {Γ' τ} (e : Exp Γ τ) (s : Sub Γ Γ') :
+    ExpP e → SubP s → SubP (Push e s).
+
+Derive Signature for SubP.
+
+Lemma ExpP_P {τ} {e : Γ ⊢ τ} : ExpP e → P e.
+Proof. intros; induction τ; simpl in *; simp ExpP in H; now reduce. Qed.
+
+End Log.
+
+Definition SN {Γ τ} : Γ ⊢ τ → Prop := ExpP (@halts Γ).
+Arguments SN {Γ τ} _ /.
+
+Definition SN_Sub {Γ Γ'} : Sub Γ' Γ → Prop := SubP (@halts Γ').
+Arguments SN_Sub {Γ Γ'} /.
+
+Definition SN_halts {Γ τ} {e : Γ ⊢ τ} : SN e → halts e := ExpP_P _.
 
 Lemma step_preserves_SN {Γ τ} {e e' : Γ ⊢ τ} :
   (e ---> e') → SN e → SN e'.
 Proof.
   intros.
-  induction τ; simp SN in *;
+  induction τ; simpl in *; simp SN in *;
   pose proof H as H1;
   apply step_preserves_halting in H1; intuition.
   - eapply IHτ1; eauto.
@@ -191,7 +215,7 @@ Lemma step_preserves_SN' {Γ τ} {e e' : Γ ⊢ τ} :
   (e ---> e') → SN e' → SN e.
 Proof.
   intros.
-  induction τ; simp SN in *;
+  induction τ; simpl in *; simp SN in *;
   pose proof H as H1;
   apply step_preserves_halting in H1; intuition.
   - eapply IHτ1; eauto.
@@ -210,22 +234,240 @@ Proof.
   now eapply step_preserves_SN'; eauto.
 Qed.
 
-Lemma multistep_App2 {Γ dom cod} {e e' : Γ ⊢ dom} {v : Γ ⊢ (dom ⟶ cod)} :
-  ValueP v → (e --->* e') → APP v e --->* APP v e'.
+Lemma multistep_Seq {Γ τ} {e1 : Γ ⊢ τ} {τ'} {e2 : Γ ⊢ τ'} :
+  Seq e1 e2 --->* e2.
 Proof.
   intros.
-  induction H.
+  eapply multi_step; eauto.
+  - now constructor.
   - now apply multi_refl.
-  - eapply multi_step; eauto.
+Qed.
+
+Ltac simpl_multistep :=
+  intros;
+  match goal with
+  | [ H : _ --->* _ |- _ ] => induction H
+  end;
+  [ now apply multi_refl
+  | eapply multi_step; eauto;
+    now constructor ].
+
+Lemma multistep_If {Γ} {e1 e1' : Γ ⊢ TyBool} {τ} {e2 e3 : Γ ⊢ τ} :
+  (e1 --->* e1') → If e1 e2 e3 --->* If e1' e2 e3.
+Proof. now simpl_multistep. Qed.
+
+Lemma multistep_Pair1 {Γ τ1 τ2} {e1 e1' : Γ ⊢ τ1} {e2 : Γ ⊢ τ2} :
+  (e1 --->* e1') → Pair e1 e2 --->* Pair e1' e2.
+Proof. now simpl_multistep. Qed.
+
+Lemma multistep_Pair2 {Γ τ1 τ2} {e1 : Γ ⊢ τ1} {e2 e2' : Γ ⊢ τ2} :
+  ValueP e1 → (e2 --->* e2') → Pair e1 e2 --->* Pair e1 e2'.
+Proof. now simpl_multistep. Qed.
+
+Lemma multistep_Pair {Γ τ1 τ2} {e1 e1' : Γ ⊢ τ1} {e2 e2' : Γ ⊢ τ2} :
+  ValueP e1' →
+  (e1 --->* e1') → (e2 --->* e2') → Pair e1 e2 --->* Pair e1' e2'.
+Proof.
+  intros.
+  induction H; intros.
+  - now apply multistep_Pair2; auto.
+  - rewrite <- IHmulti; auto.
+    apply multistep_Pair1; auto.
+    now econstructor; eauto.
+Qed.
+
+Lemma multistep_Fst1 {Γ τ1 τ2} {p p' : Γ ⊢ (τ1 × τ2)} :
+  (p --->* p') → Fst p --->* Fst p'.
+Proof. now simpl_multistep. Qed.
+
+Lemma multistep_FstPair {Γ τ1 τ2} {e1 e1' : Γ ⊢ τ1} {e2 e2' : Γ ⊢ τ2} :
+  ValueP e1' → (e1 --->* e1') →
+  ValueP e2' → (e2 --->* e2') → Fst (Pair e1 e2) --->* e1'.
+Proof.
+  intros.
+  induction H; intros.
+  - induction H0; intros.
+    + apply multi_R.
+      now constructor.
+    + rewrite <- IHmulti at 2; auto.
+      apply multistep_Fst1.
+      apply multistep_Pair; eauto.
+      constructor.
+      now apply multi_R.
+  - rewrite <- IHmulti; auto.
+    apply multistep_Fst1; auto.
+    apply multistep_Pair1; auto.
+    now apply multi_R.
+Qed.
+
+Lemma multistep_Snd1 {Γ τ1 τ2} {p p' : Γ ⊢ (τ1 × τ2)} :
+  (p --->* p') → Snd p --->* Snd p'.
+Proof. now simpl_multistep. Qed.
+
+Lemma multistep_SndPair {Γ τ1 τ2} {e1 e1' : Γ ⊢ τ1} {e2 e2' : Γ ⊢ τ2} :
+  ValueP e1' → (e1 --->* e1') →
+  ValueP e2' → (e2 --->* e2') → Snd (Pair e1 e2) --->* e2'.
+Proof.
+  intros.
+  induction H; intros.
+  - induction H0; intros.
+    + apply multi_R.
+      now constructor.
+    + rewrite <- IHmulti; auto.
+      apply multistep_Snd1.
+      apply multistep_Pair; eauto.
+      constructor.
+      now apply multi_R.
+  - rewrite <- IHmulti; auto.
+    apply multistep_Snd1; auto.
+    apply multistep_Pair1; auto.
+    now apply multi_R.
+Qed.
+
+Lemma multistep_Cons1 {Γ τ} {x x' : Γ ⊢ τ} {xs : Γ ⊢ (TyList τ)} :
+  (x --->* x') → Cons x xs --->* Cons x' xs.
+Proof. now simpl_multistep. Qed.
+
+Lemma multistep_Cons2 {Γ τ} {x : Γ ⊢ τ} {xs xs' : Γ ⊢ (TyList τ)} :
+  ValueP x → (xs --->* xs') → Cons x xs --->* Cons x xs'.
+Proof. now simpl_multistep. Qed.
+
+Lemma multistep_Cons {Γ τ} {e1 e1' : Γ ⊢ τ} {e2 e2' : Γ ⊢ (TyList τ)} :
+  ValueP e1' →
+  (e1 --->* e1') → (e2 --->* e2') → Cons e1 e2 --->* Cons e1' e2'.
+Proof.
+  intros.
+  induction H; intros.
+  - now apply multistep_Cons2; auto.
+  - rewrite <- IHmulti; auto.
+    apply multistep_Cons1; auto.
+    now econstructor; eauto.
+Qed.
+
+Lemma multistep_Car1 {Γ τ} {d d' : Γ ⊢ τ} {xs : Γ ⊢ (TyList τ)} :
+  (d --->* d') → Car d xs --->* Car d' xs.
+Proof. now simpl_multistep. Qed.
+
+Lemma multistep_Car2 {Γ τ} {d : Γ ⊢ τ} {xs xs' : Γ ⊢ (TyList τ)} :
+  ValueP d → (xs --->* xs') → Car d xs --->* Car d xs'.
+Proof. now simpl_multistep. Qed.
+
+Lemma multistep_Car {Γ τ} {d d' : Γ ⊢ τ} {xs xs' : Γ ⊢ (TyList τ)} :
+  ValueP d' →
+  (d --->* d') → (xs --->* xs') → Car d xs --->* Car d' xs'.
+Proof.
+  intros.
+  induction H; intros.
+  - now apply multistep_Car2.
+  - rewrite <- IHmulti; eauto.
+    apply multistep_Car1; auto.
+    now econstructor; eauto.
+Qed.
+
+Lemma multistep_CarNil {Γ τ} {d d' : Γ ⊢ τ} {xs : Γ ⊢ (TyList τ)} :
+  ValueP d' → (d --->* d') →
+  (xs --->* Nil) → Car d xs --->* d'.
+Proof.
+  intros.
+  dependent induction H.
+  - erewrite multistep_Car2; eauto.
+    apply multi_R.
+    now constructor.
+  - rewrite <- IHmulti; eauto.
+    apply multistep_Car1.
+    now apply multi_R.
+Qed.
+
+Lemma multistep_CarCons {Γ τ} {d e1 : Γ ⊢ τ} {e2 xs : Γ ⊢ (TyList τ)} :
+  ValueP d → ValueP e1 → ValueP e2 →
+  (xs --->* Cons e1 e2) → Car d xs --->* e1.
+Proof.
+  intros.
+  dependent induction H.
+  - erewrite multistep_Car2; eauto.
+    + apply multi_R.
+      now constructor; eauto.
+    + now constructor; eauto.
+  - specialize (IHmulti L _ _ d _ _ _ X X0 X1
+                        eq_refl JMeq_refl JMeq_refl JMeq_refl).
+    rewrite <- IHmulti; auto.
+    apply multistep_Car2; auto.
+    now apply multi_R.
+Fail Qed.
+Admitted.
+
+Lemma multistep_Cdr1 {Γ τ} {xs xs' : Γ ⊢ (TyList τ)} :
+  (xs --->* xs') → Cdr xs --->* Cdr xs'.
+Proof. now simpl_multistep. Qed.
+
+Lemma multistep_CdrNil {Γ τ} {xs : Γ ⊢ (TyList τ)} :
+  (xs --->* Nil) → Cdr xs --->* Nil.
+Proof.
+  intros.
+  dependent induction H.
+  - apply multi_R.
+    now constructor.
+  - rewrite <- IHmulti; eauto.
+    apply multi_R.
     now constructor.
 Qed.
 
-Inductive SN_Sub : ∀ {Γ Γ'}, Sub Γ' Γ → Prop :=
-  | NoSub_SN {Γ} : SN_Sub (NoSub (Γ:=Γ))
-  | Push_SN {Γ Γ' τ} (e : Exp Γ' τ) (s : Sub Γ' Γ) :
-    SN e → SN_Sub s → SN_Sub (Push e s).
+Lemma multistep_CdrCons {Γ τ} {e1 : Γ ⊢ τ} {e2 xs : Γ ⊢ (TyList τ)} :
+  ValueP e1 → ValueP e2 →
+  (xs --->* Cons e1 e2) → Cdr xs --->* e2.
+Proof.
+  intros.
+  dependent induction H.
+  - apply multi_R.
+    now constructor.
+  - specialize (IHmulti L _ _ _ _ y X X0
+                        eq_refl JMeq_refl JMeq_refl JMeq_refl).
+    rewrite <- IHmulti.
+    apply multistep_Cdr1.
+    now apply multi_R.
+Fail Qed.
+Admitted.
 
-Lemma SubExp_SN {Γ Γ'} (env : Sub Γ' Γ) τ (e : Exp Γ τ) :
+(*
+Lemma multistep_CdrCons {Γ τ} {e1 e1' : Γ ⊢ τ} {e2 e2' : Γ ⊢ (TyList τ)} :
+  ValueP e1' → (e1 --->* e1') →
+  ValueP e2' → (e2 --->* e2') → Cdr (Cons e1 e2) --->* e2'.
+Proof.
+  intros.
+  induction H; intros.
+  - induction H0; intros.
+    + apply multi_R.
+      now constructor.
+    + rewrite <- IHmulti; auto.
+      apply multistep_Cdr1.
+      apply multistep_Cons2; eauto.
+      now apply multi_R.
+  - rewrite <- IHmulti; auto.
+    apply multistep_Cdr1; auto.
+    apply multistep_Cons1; auto.
+    now apply multi_R.
+Qed.
+*)
+
+Lemma multistep_App2 {Γ dom cod} {e e' : Γ ⊢ dom} {v : Γ ⊢ (dom ⟶ cod)} :
+  ValueP v → (e --->* e') → APP v e --->* APP v e'.
+Proof. now simpl_multistep. Qed.
+
+#[export]
+Program Instance multi_Step_respects {Γ τ} :
+  Proper (multi Step --> multi Step ==> impl) (multi (Step (Γ:=Γ) (τ:=τ))).
+Next Obligation.
+  generalize dependent y0.
+  generalize dependent y.
+  induction H1; intros; eauto;
+  unfold flip in *.
+  - now transitivity x.
+  - pose proof (multi_step _ _ _ _ H H1).
+    pose proof (multi_trans _ _ _ _ H0 H3).
+    now transitivity z.
+Qed.
+
+Lemma SubExp_SN {Γ Γ'} (env : Sub Γ' Γ) {τ} (e : Exp Γ τ) :
   SN_Sub env →
   SN (SubExp env e).
 Proof.
@@ -237,18 +479,71 @@ Proof.
   - now eexists; repeat constructor.
   - now eexists; repeat constructor.
   - now eexists; repeat constructor.
-  - admit.
-  - admit.
+  - destruct (SN_halts (IHe1 env H)) as [v [P [Q]]].
+    apply (multistep_preserves_SN'
+             (e':=If v (SubExp env e2) (SubExp env e3))); auto.
+    + now apply multistep_If.
+    + inv Q; simpl.
+      * apply (step_preserves_SN' (e':=SubExp env e2)); auto.
+        now constructor.
+      * apply (step_preserves_SN' (e':=SubExp env e3)); auto.
+        now constructor.
+  - split.
+    + destruct (SN_halts (IHe1 env H)) as [v1 [P1 [Q1]]].
+      destruct (SN_halts (IHe2 env H)) as [v2 [P2 [Q2]]].
+      exists (Pair v1 v2).
+      split.
+      * now apply multistep_Pair.
+      * now repeat constructor.
+    + split.
+      * destruct (SN_halts (IHe1 env H)) as [v1 [P1 [Q1]]].
+        destruct (SN_halts (IHe2 env H)) as [v2 [P2 [Q2]]].
+        apply (multistep_preserves_SN' (e':=v1)); auto.
+        ** now eapply multistep_FstPair; eauto.
+        ** apply (multistep_preserves_SN (e:=SubExp env e1));
+           now intuition.
+      * destruct (SN_halts (IHe1 env H)) as [v1 [P1 [Q1]]].
+        destruct (SN_halts (IHe2 env H)) as [v2 [P2 [Q2]]].
+        apply (multistep_preserves_SN' (e':=v2)); auto.
+        ** now eapply multistep_SndPair; eauto.
+        ** apply (multistep_preserves_SN (e:=SubExp env e2));
+           now intuition.
   - now destruct (IHe env H).
   - now destruct (IHe env H).
   - now eexists; repeat constructor.
-  - admit.
-  - admit.
-  - admit.
-  - admit.
+  - destruct (SN_halts (IHe1 env H)) as [v1 [P1 [Q1]]].
+    destruct (SN_halts (IHe2 env H)) as [v2 [P2 [Q2]]].
+    exists (Cons v1 v2).
+    split.
+    * now apply multistep_Cons.
+    * now repeat constructor.
+  - destruct (SN_halts (IHe1 env H)) as [v1 [P1 [Q1]]].
+    destruct (SN_halts (IHe2 env H)) as [v2 [P2 [Q2]]].
+    inv Q2.
+    + apply (multistep_preserves_SN' (e':=v1)); auto.
+      * now eapply multistep_CarNil.
+      * apply (multistep_preserves_SN (e:=SubExp env e1));
+        now intuition.
+    + apply (multistep_preserves_SN' (e':=x)); auto.
+      * erewrite multistep_Car1; eauto.
+        now eapply multistep_CarCons; eauto.
+      * admit.
+  - destruct (SN_halts (IHe env H)) as [v [P [Q]]].
+    inv Q.
+    + exists Nil.
+      split.
+      * now apply multistep_CdrNil.
+      * now repeat constructor.
+    + exists xs.
+      split.
+      * now eapply multistep_CdrCons; eauto.
+      * now repeat constructor.
+  - eapply step_preserves_SN'; eauto.
+    now constructor.
   - induction env.
     + now inv v.
-    + inv H.
+    + simpl in *.
+      inv H.
       now dependent elimination v; simp SubVar.
   - eexists.
     + now eexists; repeat constructor.
@@ -267,13 +562,19 @@ Proof.
   - now apply IHe1, IHe2.
 Admitted.
 
-Theorem strong_normalization {τ} (e : Exp [] τ) : SN e.
+Theorem Exp_SN {τ} (e : Exp [] τ) : SN e.
 Proof.
   intros.
   replace e with (SubExp (Γ:=[]) NoSub e).
     apply SubExp_SN.
     now constructor.
   now rewrite NoSub_idSub, SubExp_idSub.
+Qed.
+
+Corollary strong_normalization {τ} (e : Exp [] τ) : e ⇓.
+Proof.
+  pose proof (Exp_SN e).
+  induction τ; now simpl in H.
 Qed.
 
 End Norm.
